Fixed contracts

examples/tutorial/4-bir-to-arm/tutorial_bir_to_armScript.sml
@@ -18,7 +18,8 @@ val ly_var = ``(m.REG 3w)``;
 val lx_var = ``(m.REG 2w)``;
 
 val arm8_add_reg_pre_def = Define `arm8_add_reg_pre m =
-  ((^x_var) >= 0w)
+  ((^x_var) >= 0w) /\
+  ((^x_var = ^lx_var) /\ (^y_var = ^ly_var))
 `;
 val arm8_add_reg_post_def = Define `arm8_add_reg_post m =
   ((^x_var+^y_var) = (^ly_var))
@@ -43,8 +44,9 @@ val bir_add_reg_post_def = Define `bir_add_reg_post =
 ^(beq (bplus(get_y, get_x), get_ly))`;
 
 
-val original_add_reg_loop_condition = 
- (bnot (bsle(get_lx, bconst64 0)));
+val original_add_reg_loop_condition =  (bnot (bsle(get_lx, bconst64 0)));
+
+(* Note: "BIR cjmp exits the loop is `C`, where C is the BIR ump condition*)
 val bir_add_reg_loop_condition =  bnot ``(BExp_BinExp BIExp_Or
                        (BExp_UnaryExp BIExp_Not
                           (BExp_BinPred BIExp_Equal
@@ -55,7 +57,8 @@ val bir_add_reg_loop_condition =  bnot ``(BExp_BinExp BIExp_Or
 
 val bir_add_reg_I_def = Define `bir_add_reg_I =
 ^(bandl [
-      (beq (bplus(get_y, get_x), bplus(get_ly, get_lx))),
+   (beq (bplus(get_y, get_x), bplus(get_ly, get_lx))),
+   (bsle(bconst64 0, get_lx)),
    (beq (original_add_reg_loop_condition, bir_add_reg_loop_condition))
    ])
 `;
@@ -73,9 +76,8 @@ val bir_add_reg_contract_1_post_def = Define `bir_add_reg_contract_1_post =
 
 (* contract two: loop body *)
 (* from loop body start to cjmp *)
-(* Note: "BIR cjmp exits the loop is `C`, not `not C`" *)
 val bir_add_reg_contract_2_pre_def = Define `bir_add_reg_contract_2_pre =
-^(band(``bir_add_reg_I``, bnot bir_add_reg_loop_condition))
+^(band(``bir_add_reg_I``, bir_add_reg_loop_condition))
 `;
 val bir_add_reg_contract_2_post_def = Define `bir_add_reg_contract_2_post =
  bir_add_reg_I
@@ -83,23 +85,66 @@ val bir_add_reg_contract_2_post_def = Define `bir_add_reg_contract_2_post =
 
 (* contract three: loop continue *)
 (* from cjmp to loop body start *)
-(* Note: "BIR cjmp exits the loop is `C`, not `not C`" *)
 val bir_add_reg_contract_3_pre_def = Define `bir_add_reg_contract_3_pre =
-^(band(``bir_add_reg_I``, bnot bir_add_reg_loop_condition))
+^(band(``bir_add_reg_I``, bir_add_reg_loop_condition))
 `;
 val bir_add_reg_contract_3_post_def = Define `bir_add_reg_contract_3_post =
- ^(band(``bir_add_reg_I``, bnot bir_add_reg_loop_condition))
+ ^(band(``bir_add_reg_I``, bir_add_reg_loop_condition))
 `;
 
 (* contract four: loop exit *)
 (* from cjmp to end of function except ret and sp operations *)
-(* Note: "BIR cjmp exits the loop is `C`, not `not C`" *)
 val bir_add_reg_contract_4_pre_def = Define `bir_add_reg_contract_4_pre =
-^(band(``bir_add_reg_I``, bir_add_reg_loop_condition))
+^(band(``bir_add_reg_I``, bnot bir_add_reg_loop_condition))
 `;
 val bir_add_reg_contract_4_post_def = Define `bir_add_reg_contract_4_post =
  bir_add_reg_post
 `;
+
+
+
+(* Here we prove that the contracts transfer properties between the two models *)
+(* We first show that the bir contract is a boolean property *)
+val bir_add_reg_pre_is_bool_pred_thm = prove(
+  ``bir_is_bool_exp bir_add_reg_pre``,
+  FULL_SIMP_TAC (std_ss++bir_is_bool_ss) [bir_add_reg_pre_def]
+);
+
+val arm_to_bir_exp_thms = (((CONJUNCTS o UNDISCH o fst o EQ_IMP_RULE) bir_lifting_machinesTheory.arm8_bmr_rel_EVAL) @
+  [bir_expTheory.bir_eval_bin_exp_REWRS, bir_immTheory.type_of_bir_imm_def,
+         bir_exp_immTheory.bir_bin_exp_REWRS, bir_exp_immTheory.bir_bin_exp_GET_OPER_def] @
+  [bir_expTheory.bir_eval_bin_pred_REWRS, bir_immTheory.type_of_bir_imm_def,
+         bir_exp_immTheory.bir_bin_pred_REWRS, bir_exp_immTheory.bir_bin_pred_GET_OPER_def,
+         bir_immTheory.bool2b_def] @
+  [(UNDISCH o (SPECL [``bs:bir_state_t``, ``ms:arm8_state``])) bload_64_to_arm8_load_64_thm] @
+  [bir_bool_expTheory.BVal_Imm_bool2b_EQ_TF_REWRS, bir_valuesTheory.BType_Bool_def ] @
+  [bir_expTheory.bir_eval_exp_def] @ [bir_expTheory.bir_eval_unary_exp_REWRS,
+  bir_exp_immTheory.bir_unary_exp_GET_OPER_def,  bir_exp_immTheory.bir_unary_exp_REWRS] @
+  [bool2w_def, bir_bool_expTheory.bir_val_true_def]);
+
+
+(* Then we show that the arm precondition entails the bir precondition *)
+val arm8_pre_imp_bir_pre_thm = store_thm("arm8_pre_imp_bir_pre_thm", 
+``bir_pre_arm8_to_bir arm8_add_reg_pre bir_add_reg_pre``
+,
+FULL_SIMP_TAC (std_ss) [bir_pre_arm8_to_bir_def, bir_add_reg_pre_is_bool_pred_thm] >>
+REPEAT STRIP_TAC >>
+SIMP_TAC (std_ss) [bir_add_reg_pre_def] >>
+SIMP_TAC (std_ss) arm_to_bir_exp_thms >>
+EVAL_TAC >>
+UNDISCH_TAC ``arm8_add_reg_pre ms`` >>
+FULL_SIMP_TAC (std_ss) [arm8_add_reg_pre_def] >>
+Q.ABBREV_TAC `a = ms.REG 2w` >>
+Q.ABBREV_TAC `b = ms.REG 3w` >>
+Q.ABBREV_TAC `c = ms.REG 4w` >>
+Q.ABBREV_TAC `d = ms.REG 5w` >>
+(fn (asl,goal) => ASSUME_TAC (HolSmtLib.Z3_ORACLE_PROVE  goal)(asl,goal)) >>
+FULL_SIMP_TAC std_ss []
+);
+
+
+
+
 
 
 
@@ -114,11 +159,7 @@ EVAL ``arm8_wf_varset (bir_vars_of_exp bir_add_reg_contract_1_pre)``;
 
 
 
-val bir_I_is_bool_pred_thm = prove(
-  ``bir_is_bool_exp b_sqrt_I``,
 
-FULL_SIMP_TAC (std_ss++bir_is_bool_ss) [b_sqrt_I_def]
-);
 
 val arm8I_imp_bI_thm = store_thm("arm8I_imp_bI_thm", 
 ``bir_pre_arm8_to_bir arm8_sqrt_I b_sqrt_I``
